ass2/ex3.dfy
@@ -1,4 +1,17 @@
 predicate ooo(s:seq<int>)
+requires |s| >= 2;
 {
- true
+  exists i | 0 <= i < |s| :: if i == 0 then s[i] !in s[i+1..|s|] else s[i] !in s[0..i] + s[i+1..|s|]
+}
+
+method Main()
+{
+  var s := [1,1,42,1];
+  assert s[0]==1 && s[1]==1 && s[2]==42 && s[3]==1;
+  assert ooo(s); // Part (i)
+
+  var s1 := [1,1,42,42];
+  assert s1[0]==1 && s1[1]==1 && s1[2]==42 && s1[3]==42;
+  assert !ooo(s1);
+
 }
