ass2/QuackRepair.dfy
@@ -1,0 +1,111 @@
+class Quack
+{
+    var buf:array<char>;
+    var m:int, n:int;
+
+    ghost var shadow: seq<char>;
+
+    predicate Valid() reads this, this.buf
+    { buf.Length!=0 && 0<=m<=n<=buf.Length && shadow==buf[m..n] }
+
+    constructor(size: int)
+    requires size > 0;
+    ensures shadow == []
+    ensures fresh(buf)
+    ensures Valid()
+    {
+        buf := new char[size];
+        m, n:= 0, 0;
+        shadow:= [];
+    }
+
+    method Empty() returns (x: bool)
+    requires Valid();
+    ensures x <==> shadow==[] // an empty shadow means x is true
+    ensures Valid()           // can be better to make this last
+    {
+       x := m==n;             // no elements means x is true
+    }
+
+    method Push(x: char) modifies this, this.buf, this`m, this`n
+    requires Valid();
+    // code
+    ensures if old(n)   == old(buf.Length) then fresh(buf) else buf==old(buf)
+    ensures if old(n-m) == old(buf.Length) then buf.Length==2*old(buf.Length) else buf.Length==old(buf.Length)
+    ensures 0<n<=buf.Length ==> buf[n-1]==x
+    // shadow
+    ensures |shadow|    == |old(shadow)|+1
+    ensures   shadow    == old(shadow) + [x]; // new tail
+    ensures Valid()
+    {
+        if n==buf.Length
+        {
+            var b:= new char[buf.Length];          // temporary
+            if m==0 { b:= new char[2*buf.Length]; }// double size
+            forall (i | 0<=i<n-m) { b[i]:= buf[m+i]; } // copy m..n to 0..n-m
+            buf, m, n:= b, 0, n-m;                     // copy b to buf, reset m,n
+        }
+        buf[n], n:= x, n+1;         // now we definitely have room
+        shadow:= shadow + [x];      // same as previous slide: concat 'x'
+    }
+
+    method Pop() returns(x: char) modifies this, this`n
+    requires Valid()
+    requires  shadow != []
+    // code
+    ensures   buf    == old(buf)                  // buf name does not change
+    ensures   x      == old(buf[n-1])             // element n-1 is returned
+    ensures   n      == old(n-1)                  // n moves down
+    // shadow
+    ensures |shadow| == |old(shadow)|-1           // popped an elem
+    ensures   x      == old(shadow[|shadow|-1])   // last element
+    ensures shadow   == old(shadow[..|shadow|-1]) // chop off tail
+    ensures Valid()                               // check okay at end
+    {
+        x, n:= buf[n-1], n-1;                     // get tail, decr n
+        shadow:= shadow[..|shadow|-1];            // chop tail off shadow
+    }
+///////////////////////////////////////////////////////
+    // DO NOT CHANGE ANYTHING ABOVE THIS LINE //
+    ////////////////////////////////////////////
+
+
+method Repair(i:nat, c:char)
+requires i <= this.buf.Length;
+{
+
+}
+
+
+
+
+    ////////////////////////////////////////////
+    // DO NOT CHANGE ANYTHING BELOW THIS LINE //
+///////////////////////////////////////////////////////
+
+} // end of Quack class
+
+method Tester()
+{
+    var q:= new Quack(6);
+    var p: char;
+    var e: bool;
+
+    q.Push('m');
+    q.Push('a');
+    q.Push('k');
+    q.Push('e');
+    q.Repair(0, 'o');                 // e --> o
+    p := q.Pop();    assert p=='o';
+    q.Repair(2, 'y');                 // m --> y
+    p := q.Pop();    assert p=='k';
+    q.Repair(3, 'x');                 // bad repair, ignored
+    q.Repair(0, 'a');                 // k --> a
+    p := q.Pop();    assert p=='a';
+    q.Repair(2, 'x');                 // bad repair, ignored
+    q.Repair(1, 'x');                 // bad repair, ignored
+    p := q.Pop();    assert p=='y';
+
+    e := q.Empty();  assert e;
+    q.Repair(0, 'x');                 // bad repair, ignored
+}
