ass2/ex5.dfy
@@ -1,0 +1,8 @@
+method Prison(all: set<nat>, inlight:bool) returns (swch: set<nat>)
+requires |all| > 1
+ensures |swch|+1 == |all|
+ensures swch < all
+decreases *
+{
+
+}
